Update goose tests

src/goose_lang/examples/goose_semantics.v
@@ -329,6 +329,30 @@ Definition failing_testFunctionOrdering: val :=
                 then #false
                 else (struct.get Pair.S "x" "p" + struct.get Pair.S "x" "q" = #109)))))))).
 
+(* int_conversions.go *)
+
+Definition testU64ToU32: val :=
+  rec: "testU64ToU32" <> :=
+    let: "ok" := ref_to boolT #true in
+    let: "x" := #1230 in
+    let: "y" := #(U32 1230) in
+    "ok" <-[boolT] (![boolT] "ok") && (to_u32 "x" = "y");;
+    "ok" <-[boolT] (![boolT] "ok") && (to_u64 "y" = "x");;
+    ![boolT] "ok".
+
+Definition testU32Len: val :=
+  rec: "testU32Len" <> :=
+    let: "s" := NewSlice byteT #100 in
+    (to_u32 (slice.len "s") = #(U32 100)).
+
+Definition Uint32: ty := uint32T.
+
+(* https://github.com/tchajed/goose/issues/14 *)
+Definition failing_testU32NewtypeLen: val :=
+  rec: "failing_testU32NewtypeLen" <> :=
+    let: "s" := NewSlice byteT #20 in
+    (slice.len "s" = #(U32 20)).
+
 (* lock.go *)
 
 (* We can't interpret multithreaded code, so this just checks that
