src/goose_lang/interpreter/generated_test.v
@@ -34,6 +34,11 @@ Example testEncDec64_ok : testEncDec64 #() ~~> #true := t.
 (* function_ordering.go *)
 Fail Example testFunctionOrdering_ok : failing_testFunctionOrdering #() ~~> #true := t.
 
+(* int_conversions.go *)
+Example testU64ToU32_ok : testU64ToU32 #() ~~> #true := t.
+Example testU32Len_ok : testU32Len #() ~~> #true := t.
+Fail Example testU32NewtypeLen_ok : failing_testU32NewtypeLen #() ~~> #true := t.
+
 (* lock.go *)
 Example testsUseLocks_ok : testsUseLocks #() ~~> #true := t.
 
